developing entailment lemmas

src/definitions.lean
@@ -4,11 +4,10 @@ Definitions of a type theory
 Author: Billy Price
 -/
 import data.finset
-import tactic
 namespace TT
 
 inductive type : Type
-| Unit | Omega | Prod (A B : type)| Pow (A : type)
+| Unit | Omega | Prod (A B : type) | Pow (A : type)
 
 notation `Ω` := type.Omega
 notation `𝟙` := type.Unit
@@ -45,7 +44,7 @@ infixr ` ⋀ ` :70 := term.and -- input \And or \bigwedge
 infixr ` ⋁ ` :59 := term.or  -- input \Or or \bigvee
 
 def not (p : term) := p ⟹ ⊥
-prefix `∼`:max := not -- input \~
+instance term_has_neg : has_neg term := ⟨not⟩
 
 def iff (p q: term) := (p ⟹ q) ⋀ (q ⟹ p)
 infix ` ⇔ `:60 := iff -- input \<=>
@@ -64,6 +63,9 @@ notation `∃[` Q:(foldr `,` (A q, λ p : term, ∃' A (q p)) id) `]` := Q
 
 section substitution
 
+  variables {x p q a α b φ : term}
+  variable {A : type}
+
   @[simp]
   def lift (d : ℕ) : ℕ → term → term
   | k ⁎          := ⁎
@@ -81,6 +83,19 @@ section substitution
   
   notation `^` := lift 1 0
 
+  @[simp] lemma lift_star : ^⁎ = ⁎ := rfl
+  @[simp] lemma lift_top : ^⊤ = ⊤ := rfl
+  @[simp] lemma lift_bot : ^⊥ = ⊥ := rfl
+  @[simp] lemma lift_and : ^(p ⋀ q) = ^p ⋀ ^q := rfl
+  @[simp] lemma lift_or : ^(p ⋁ q) = ^p ⋁ ^q := rfl
+  @[simp] lemma lift_imp : ^(p ⟹ q) = ^p ⟹ ^q := rfl
+  @[simp] lemma lift_elem : ^(a ∈ α) = (^a ∈ ^α) := rfl
+  @[simp] lemma lift_pair : ^(⟪a,b⟫) = ⟪^a,^b⟫ := rfl
+  @[simp] lemma lift_var {n : ℕ} : ^↑n = ↑(n+1) := rfl
+  
+  @[simp] lemma lift_zero {k : ℕ} {a : term} : lift 0 k a = a :=
+  by induction a generalizing k; simp *
+
   @[simp]
   def subst : ℕ → term → term → term
   | n x ⁎          := ⁎
@@ -96,33 +111,16 @@ section substitution
   | n x (∀' A φ)   := ∀' A (subst (n+1) (^ x) φ)
   | n x (∃' A φ)   := ∃' A (subst (n+1) (^ x) φ)
 
+  notation  φ`⁅`:max b // n`⁆` := subst n b φ
+  notation  φ`⁅`:max b `⁆` := φ⁅ b // 0⁆
+
   @[simp]
-  lemma subst_id {a : term} {n : ℕ} : subst n (↑n) a = a :=
+  lemma subst_id {a : term} {n : ℕ} : a⁅↑n // n⁆ = a :=
   begin
-    induction a generalizing n;simp * at *,
-    case term.var : m {split_ifs, rw h, refl, refl},
-    all_goals {exact a_ih}
+    induction a generalizing n,
+    case term.var : m {simp, split_ifs, rw h, refl, refl},
+    all_goals {simp *},
   end
-
-  notation  `⁅` φ ` // `  b `⁆` := subst 0 b φ
-
-  #reduce ⁅ ↑0 // ⊤ ⋀ ⊥⁆
-  #reduce ⁅ ↑1 // ⊤ ⋀ ⊥⁆
-
-  def FV : term → finset ℕ
-  | ⁎          := ∅
-  | ⊤          := ∅
-  | ⊥          := ∅
-  | (p ⋀ q)    := FV p ∪ FV q
-  | (p ⋁ q)    := FV p ∪ FV q
-  | (p ⟹ q)  := FV p ∪ FV q
-  | (a ∈ α)    := FV a ∪ FV α
-  | ⟪a,b⟫      := FV a ∪ FV b
-  | (var n)    := {n}
-  | ⟦ A | φ ⟧   := ((FV φ).erase 0).image nat.pred
-  | (∀' A φ)   := ((FV φ).erase 0).image nat.pred
-  | (∃' A φ)   := ((FV φ).erase 0).image nat.pred
-
 end substitution
 
 def term_eq (A:type) (a₁ a₂ : term) : term := ∀' (𝒫 A) $ ((^ a₁) ∈ ↑0) ⇔ ((^ a₂) ∈ ↑0)
@@ -145,9 +143,10 @@ def term_prod (A B : type) (α β : term) : term :=
 
 -- * * * * * * * * * * * * * * * * * * * * * * * * * * * * * * * * * * * * * * *
 open list
-local notation l₁ ++ l₂ := list.append l₁ l₂
 
 def context := list type
+
+instance context_has_append : has_append context := ⟨list.append⟩
 
 inductive WF : context → type → term → Prop
 | star {Γ}         : WF Γ 𝟙 ⁎
@@ -168,19 +167,19 @@ def closed : type → term → Prop := WF list.nil
 /-! ### entails -/
 
 inductive entails : context → term → term → Prop
-| axm        {Γ} {p}       : WF Γ Ω p → entails Γ p p
-| vac        {Γ} {p}       : WF Γ Ω p → entails Γ p ⊤
-| abs        {Γ} {p}       : WF Γ Ω p → entails Γ ⊥ p
-| and_intro  {Γ} {p q r}   : entails Γ p q → entails Γ p r → entails Γ p (q ⋀ r)
-| and_left   {Γ} (p q r)   : entails Γ p (q ⋀ r) → entails Γ p q
-| and_right  {Γ} (p q r)   : entails Γ p (q ⋀ r) → entails Γ p r
-| or_intro   {Γ} {p q r}   : entails Γ p r → entails Γ q r → entails Γ (p ⋁ q) r
-| or_left    {Γ} (p q r)   : entails Γ (p ⋁ q) r → entails Γ p r
-| or_right   {Γ} (p q r)   : entails Γ (p ⋁ q) r → entails Γ q r
+| axm          {Γ} {p}     : WF Γ Ω p → entails Γ p p
+| vac          {Γ} {p}     : WF Γ Ω p → entails Γ p ⊤
+| abs          {Γ} {p}     : WF Γ Ω p → entails Γ ⊥ p
+| and_intro    {Γ} {p q r} : entails Γ p q → entails Γ p r → entails Γ p (q ⋀ r)
+| and_left     {Γ} (p q r) : entails Γ p (q ⋀ r) → entails Γ p q
+| and_right    {Γ} (p q r) : entails Γ p (q ⋀ r) → entails Γ p r
+| hyp_or       {Γ} {p q r} : entails Γ p r → entails Γ q r → entails Γ (p ⋁ q) r
+| hyp_or_left  {Γ} (p q r) : entails Γ (p ⋁ q) r → entails Γ p r
+| hyp_or_right {Γ} (p q r) : entails Γ (p ⋁ q) r → entails Γ q r
 | imp_to_and {Γ} {p q r}   : entails Γ p (q ⟹ r) → entails Γ (p ⋀ q) r
 | and_to_imp {Γ} {p q r}   : entails Γ (p ⋀ q) r → entails Γ p (q ⟹ r)
-| weakening  {Γ} {p q} (Δ) : entails Γ p q → entails (list.append Γ Δ) p q
-| cut        {Γ} (p c q)   : entails Γ p c → entails Γ c q → entails Γ p q
+| weakening  {p q} (K Δ Γ) : entails (K ++ Γ) p q → entails (K ++ Δ ++ Γ) (lift Δ.length K.length p) (lift Δ.length K.length q)
+| cut        {Γ} {p q} (c) : entails Γ p c → entails Γ c q → entails Γ p q
 | all_elim   {Γ} {p φ A}   : entails Γ p (∀' A φ) → entails (A::Γ) (^ p) φ
 | all_intro  {Γ} {p φ} (A) : entails (A::Γ) (^ p) φ → entails Γ p (∀' A φ)
 | ex_elim    {Γ} {p φ A}   : entails Γ p (∃' A φ) → entails (A::Γ) (^ p) φ
@@ -190,7 +189,7 @@ inductive entails : context → term → term → Prop
 | star_unique              : entails [] ⊤ $ ∀[𝟙] (↑0 ≃[𝟙] ⁎)
 | pair_rep      {A B}      : entails [] ⊤ $ ∀[A 𝕏 B] $ ∃[A,B] $ ↑2 ≃[A 𝕏 B] ⟪↑1,↑0⟫
 | pair_distinct {A B}      : entails [] ⊤ $ ∀[A,B,A,B] $ (⟪↑3,↑2⟫ ≃[A 𝕏 B] ⟪↑1,↑0⟫) ⟹ ((↑3 ≃[A] ↑1) ⋀ (↑2 ≃[B] ↑0))
-| sub      {Γ} (B) (b p q) : WF Γ B b → entails (B::Γ) p q → entails Γ (⁅p // b⁆) (⁅q // b⁆)
+| sub      {Γ} {p q} (B b) : WF Γ B b → entails (B::Γ) p q → entails Γ (p⁅b⁆) (q⁅b⁆)
 | comp     {Γ} (A) (φ)     : WF (A::Γ) Ω φ → entails Γ ⊤ (∀' A $ (↑0 ∈ (^ ⟦A | φ⟧)) ⇔ φ)
 
 prefix `⊨`:1 := entails [] ⊤
@@ -201,11 +200,11 @@ notation `⊨[` Γ:(foldr `,` (h t, list.cons h t) list.nil) `] ` ψ := entails 
 section
   variables p q φ ψ : term
 
-  #reduce   ⊨ (p ⋁ ∼p)  -- entails [] ⊤ (or p (imp p ⊥))
-  #reduce q ⊨ (p ⋁ ∼p)  -- entails [] q (or p (imp p ⊥))
+  #reduce   ⊨ (p ⋁ -p)  -- entails [] ⊤ (or p (imp p ⊥))
+  #reduce q ⊨ (p ⋁ -p)  -- entails [] q (or p (imp p ⊥))
   #reduce   ⊨[Ω,𝟙] p -- entails [Ω,⁎] ⊤ p
   #reduce q ⊨[Ω,𝟙] p -- entails [Ω,⁎] q p
-end 
+end
 
 
 end TT
