src/entails.lean
@@ -1,0 +1,84 @@
+import definitions
+import wellformedness
+import tactic
+
+namespace TT
+namespace entails
+open entails
+
+variables p q r φ ψ : term
+variable {Γ : context}
+
+lemma hyp_and_left (_ : WF Γ Ω p) (_ : WF Γ Ω q) : entails Γ (p ⋀ q) p :=
+  by {intros, apply entails.and_left _ p q, apply entails.axm, apply WF.and, tidy}
+lemma hyp_and_right (_ : WF Γ Ω p) (_ : WF Γ Ω q) : entails Γ (p ⋀ q) q :=
+  by {apply entails.and_right _ p q, apply entails.axm, apply WF.and, tidy}
+
+lemma from_imp {p q}: entails Γ ⊤ (p ⟹ q) → entails Γ p q :=
+begin
+  intro h₁, 
+  have : WF Γ Ω (p ⟹ q), from WF.entails_right h₁,
+  have wfp : WF Γ Ω p, from WF.imp_left _ _ this,
+  have wfq : WF Γ Ω q, from WF.imp_right _ _ this,
+  apply cut (⊤ ⋀ p),
+    { apply_rules and_intro,
+        { exact vac wfp },
+        { exact axm wfp}
+    },
+    { exact imp_to_and h₁ }
+end
+
+lemma to_imp {p q} : entails Γ p q → entails Γ ⊤ (p ⟹ q) :=
+begin
+  intro h₁,
+  apply_rules [and_to_imp, cut p, and_right _ ⊤ _, axm],
+  WF_prover,
+  exact WF.entails_left h₁,
+end
+
+lemma or_intro_left (p q) : WF Γ Ω p → WF Γ Ω q → entails Γ p (p ⋁ q) :=
+  by intros wfp wfq;apply hyp_or_left;apply axm;WF_prover
+lemma or_intro_right (p q) : WF Γ Ω p → WF Γ Ω q → entails Γ q (p ⋁ q) :=
+  by intros wfp wfq;apply hyp_or_right;apply axm;WF_prover
+
+def is_star {a : term} : WF Γ 𝟙 a → entails Γ ⊤ (a ≃[𝟙] ⁎) :=
+begin
+  intro wfa,
+  apply @sub _ ⊤ (↑0 ≃[𝟙] ⁎) _ _ wfa,
+  have lift_top : (⊤ : term) = ^⊤, by refl,
+  rw lift_top,
+  apply all_elim,
+  have nil_context : Γ = ([] ++ Γ ++ []), by simp,
+  rw nil_context,
+  have lift_0_top : (⊤ : term) = lift Γ.length 0 ⊤, by simp,
+  rw lift_0_top,
+  have lift_0_forall : (∀' 𝟙 (↑0 ≃[𝟙] ⁎)) = lift Γ.length 0 (∀' 𝟙 (↑0 ≃[𝟙] ⁎)), by simp; constructor,
+  rw lift_0_forall,
+  apply weakening,
+  exact star_unique
+end
+
+lemma meta_all_sub {A φ a} : WF Γ A a → entails Γ ⊤ (∀' A φ) → entails Γ ⊤ (φ⁅a⁆) :=
+begin
+  intros wfa ent_all,
+  have : (⊤ : term) =  ⊤⁅a⁆, by refl, rw this,
+  apply sub _ _ wfa,
+  have : (⊤ : term) = ^ ⊤, by refl, rw this,
+  exact all_elim ent_all
+end
+
+lemma all_sub {A φ a} : WF (A :: Γ) Ω φ → entails (A::Γ) (^ (∀' A φ)) (φ⁅a⁆) :=
+begin
+  intro wf,
+  apply cut φ,
+    { apply_rules [all_elim, axm], WF_prover },
+    {
+      induction wf; sorry
+     }
+end
+
+
+end entails
+
+
+end TT
