src/lemmas.lean
@@ -1,97 +1,33 @@
 import definitions
 import wellformedness
-import tactic
+import tactic.tidy
 
 namespace TT
 
-variables p q r φ ψ : term
-variable {Γ : context}
-
-lemma from_imp {Γ : context} : entails Γ ⊤ (q ⟹ r) → entails Γ q r :=
-begin
-  intro h₁,
-  apply entails.cut _ (⊤ ⋀ q) _,
-  apply_rules [entails.and_intro, entails.vac, entails.axm];
-    { apply @WF.imp_left _ q r,
-      exact WF.proof_right h₁
-    },
-  exact entails.imp_to_and h₁,
-end
-
-lemma to_imp {Γ : context} : entails Γ q r → entails Γ ⊤ (q ⟹ r) :=
-begin
-  intro h₁,
-  apply_rules [entails.and_to_imp, entails.cut _ q _, entails.and_right _ ⊤ _, entails.axm],
-  WF_prover,
-  apply WF.proof_left h₁,
-end
-lemma entails.or_inl (wfq : WF Γ Ω q) (prfp :entails Γ ⊤ p) : entails Γ ⊤ (p ⋁ q) :=
-  by {apply entails.cut _ p _, assumption, apply entails.or_left _ q, apply entails.axm, apply_rules [WF.or, WF.proof_right]}
-lemma entails.or_inr (wfq : WF Γ Ω p) (prfp :entails Γ ⊤ q) : entails Γ ⊤ (p ⋁ q) :=
-  by {apply entails.cut _ q _, assumption, apply entails.or_right _ q, apply entails.axm, apply_rules [WF.or, WF.proof_right]}
-
-lemma proof_of_and_left (_ : WF Γ Ω p) (_ : WF Γ Ω q) : entails Γ (p ⋀ q) p :=
-  by {intros, apply entails.and_left _ p q, apply entails.axm, apply WF.and, tidy}
-lemma proof_of_and_right (_ : WF Γ Ω p) (_ : WF Γ Ω q) : entails Γ (p ⋀ q) q :=
-  by {apply entails.and_right _ p q, apply entails.axm, apply WF.and, tidy}
-
-example (_ : WF Γ Ω p) (_ : WF Γ Ω q) : entails Γ (p ⋀ q) (q ⋀ p) :=
-begin
-  apply entails.and_intro,
-  apply proof_of_and_right,
-  tidy,
-  apply proof_of_and_left,
-  tidy
-end
-
-lemma eq_sound {A : type} {a₁ a₂ : term} (eq : ⊨ (a₁ ≃[A] a₂)) (φ : term) : entails Γ ⊤ ⁅φ // a₁⁆ → entails Γ ⊤ ⁅φ // a₂⁆ :=
+lemma eq_sound {Γ} {A : type} {a₁ a₂ : term} (eq : ⊨ (a₁ ≃[A] a₂)) (φ : term) : entails Γ ⊤ (φ⁅a₁⁆) → entails Γ ⊤ (φ⁅a₂⁆) :=
 by sorry
 
 lemma reverse_extensionality (A : type) : ⊨ (∀' (𝒫 A) $ ∀' (𝒫 A) $ (↑1 ≃[𝒫 A] ↑0) ⟹ (∀' A ((↑0 ∈ ↑2) ⇔ (↑0 ∈ ↑1)))) :=
-begin
-  apply entails.all_intro 𝒫 A,
-  apply entails.all_intro 𝒫 A,
-  apply to_imp,
-  apply from_meta_imp,
-  any_goals {apply_rules WF_rules; refl},
-  intro h,
-  sorry
-end
+by sorry
 
-def is_star {Γ : context} {a : term} : WF Γ 𝟙 a → entails Γ ⊤ (a ≃[𝟙] ⁎) :=
-begin
-  intro wfa,
-  apply entails.sub 𝟙 a ⊤ (↑0 ≃[𝟙] ⁎),
-  assumption,
-  have : (⊤ : term) = ^ ⊤, by rw WF.lift_closed; exact WF.top,
-  rw this,
-  apply entails.all_elim,
-  rw ←list.nil_append Γ,
-  apply entails.weakening,
-  exact entails.star_unique
-end
+open entails
 
-local notation `[]` := list.nil
+variables {φ ψ : term}
+variable {Γ : context}
 
-lemma phi_ent_phi_and_top (h : WF [] Ω φ): φ ⊨ (φ ⋀ ⊤) :=
-begin
-  apply entails.and_intro,
-  apply entails.axm,
-  exact h,
-  apply entails.vac,
-  exact h
-end
+lemma meta.from_ent {p} {wfP : WF [] Ω p} : entails Γ φ ψ  → entails Γ p φ → entails Γ p ψ :=
+  λ _ _, (by {apply cut φ, tidy})
 
-section meta_conversion
+lemma meta.to_ent (wfφ : WF Γ Ω φ) : (∀ p, entails Γ p φ → entails Γ p ψ) → entails Γ φ ψ :=
+  λ h, h φ (axm wfφ)
 
-lemma ent_to_meta {p} {wfP : WF [] Ω p} : entails Γ φ ψ  → entails Γ p φ → entails Γ p ψ :=
-  λ _ _, (by {apply entails.cut _ φ _, tidy})
-
-lemma meta_to_ent (wfφ : WF Γ Ω φ) : (∀ p, entails Γ p φ → entails Γ p ψ) → entails Γ φ ψ :=
-  λ h, h φ (entails.axm wfφ)
-
-end meta_conversion
-
-
+lemma meta.from_imp {p} : entails Γ p (φ ⟹ ψ) → (entails Γ p φ → entails Γ p ψ) :=
+  λ imp hpφ, (begin
+    apply cut (p ⋀ φ),
+    apply and_intro,
+      apply axm, exact WF.entails_left imp,
+      exact hpφ,
+    exact imp_to_and imp,
+  end)
 
 end TT
